Strengthen the Bag interface in preparation of the move to multisets
Replace the SetEq predicate with Permutation, and prove that these
strengthened constraints hold for the various implementations. The
proofs are much cleaner than before, but could still be refactored a
bit.

src/QueryStructure/Refinements/Bags/BagsInterface.v
@@ -1,4 +1,4 @@
-Require Export Program SetEq SetEqProperties.
+Require Export Program Permutation.
 
 Unset Implicit Arguments.
 
@@ -9,9 +9,10 @@ Definition BagInsertEnumerate
            {TContainer TItem: Type}
            (benumerate : TContainer -> list TItem)
            (binsert    : TContainer -> TItem -> TContainer) :=
-  forall item inserted container,
-    List.In item (benumerate (binsert container inserted)) <->
-    List.In item (benumerate container) \/ item = inserted.
+  forall inserted container,
+    Permutation
+      (benumerate (binsert container inserted))
+      (inserted :: (benumerate container)).
 
 Definition BagInsertCount
            {TContainer TItem}
@@ -50,7 +51,7 @@ Definition BagFindCorrect
            (bfind_matcher : TSearchTerm -> TItem -> bool)
            (benumerate : TContainer -> list TItem) :=
   forall container search_term,
-    SetEq
+    Permutation
       (List.filter (bfind_matcher search_term) (benumerate container))
       (bfind container search_term).
 
