src/QueryStructure/Refinements/Bags/BagsOfTuples.v
@@ -34,8 +34,13 @@ Proof.
   apply (ListAsBag [] (@MatchAgainstSearchTerms heading)); eauto.
 Defined.
 
-Require Import FMapAVL.
+Definition TupleListBag {heading} :=
+  {|
+    BagType        := list (@Tuple heading);
+    SearchTermType := (SearchTermsCollection heading)
+  |}.
 
+Require Import FMapAVL.
 
 Module NIndexedMap := FMapAVL.Make N_as_OT.
 Module ZIndexedMap := FMapAVL.Make Z_as_OT.
@@ -121,6 +126,7 @@ Ltac mkIndex heading attributes :=
   assert (list (@ProperAttribute heading)) as decorated_source by autoconvert (@CheckType heading);
   apply (NestedTreeFromAttributes' heading decorated_source).
 
+(*
 Require Import Beatles.
 Local Open Scope string_scope.
 
@@ -144,6 +150,7 @@ Time Eval simpl in (bfind IndexedAlbums (None, (None, (None, [TupleEqualityMatch
 
 (*Time Eval simpl in (@bfind _ _ _ (BagProof _ SampleIndex) IndexedAlbums (Some 3, (Some 1, (None, @nil (TSearchTermMatcher AlbumHeading))))).*)
 *)
+*)
 
 Require Import EnsembleListEquivalence QueryStructure InsertQSSpecs AdditionalLemmas.
 
@@ -160,10 +167,10 @@ Lemma binsert_correct_DB {TContainer TSearchTerm} :
                                    (RelationInsert tuple (GetUnConstrRelation qs index))) index)
         (benumerate (binsert store tuple)).
 Proof.
-  intros * equiv **;
-                 apply (ensemble_list_equivalence_set_eq_morphism get_update_unconstr_iff);
+  intros * equiv ** ;
+  apply (ensemble_list_equivalence_set_eq_morphism get_update_unconstr_iff);
   unfold RelationInsert, EnsembleListEquivalence, Ensembles.In in *;
   setoid_rewrite (@binsert_enumerate _ _ _ store_is_bag _);
-  setoid_rewrite <- equiv;
-  tauto.
+  simpl; setoid_rewrite <- equiv;
+  intuition.
 Qed.
